proof/crefine/ARM/StateRelation_C.thy
@@ -604,7 +604,7 @@ fun
   | "irqstate_to_C irqstate.IRQReserved = scast Kernel_C.IRQReserved"
 
 definition
-  cinterrupt_relation :: "interrupt_state \<Rightarrow> 'a ptr \<Rightarrow> (word32[160]) \<Rightarrow> bool"
+  cinterrupt_relation :: "interrupt_state \<Rightarrow> 'a ptr \<Rightarrow> (word32[irq_array_size]) \<Rightarrow> bool"
 where
   "cinterrupt_relation airqs cnode cirqs \<equiv>
      cnode = Ptr (intStateIRQNode airqs) \<and>
@@ -704,8 +704,10 @@ where
 
 context state_rel begin
 
+value_type intState_array_size = "2^irqBits :: nat"
+
 \<comment> \<open>The IRQ node is a global array of CTEs.\<close>
-abbreviation intStateIRQNode_array_Ptr :: "(cte_C[256]) ptr" where
+abbreviation intStateIRQNode_array_Ptr :: "(cte_C[intState_array_size]) ptr" where
   "intStateIRQNode_array_Ptr \<equiv> Ptr (symbol_table ''intStateIRQNode'')"
 
 \<comment> \<open>But for compatibility with older proofs (written when the IRQ Node was a global pointer
