proof/crefine/ARM_HYP/ADT_C.thy
@@ -315,8 +315,8 @@ lemma cirqstate_cancel:
 definition
   "cint_state_to_H cnode cirqs \<equiv>
    InterruptState (ptr_val cnode)
-     (\<lambda>i::10 word. if i \<le> scast ARM_HYP.maxIRQ then cirqstate_to_H (index cirqs (unat i))
-                else irqstate.IRQInactive)"
+     (\<lambda>i::irq. if i \<le> Kernel_Config.maxIRQ then cirqstate_to_H (index cirqs (unat i))
+               else irqstate.IRQInactive)"
 
 lemma cint_rel_to_H:
   "irqs_masked' s \<Longrightarrow>
@@ -325,8 +325,7 @@ lemma cint_rel_to_H:
   apply (simp add: irqs_masked'_def)
   apply (cases "ksInterruptState s")
   apply (rename_tac "fun")
-  apply (clarsimp simp: cinterrupt_relation_def cint_state_to_H_def
-                        ARM_HYP.maxIRQ_def Kernel_C.maxIRQ_def)
+  apply (clarsimp simp: cinterrupt_relation_def cint_state_to_H_def Kernel_C_maxIRQ)
   apply (rule ext)
   apply clarsimp
   apply (drule spec, erule impE, assumption)
