proof/crefine/ARM_HYP/Finalise_C.thy
@@ -970,6 +970,26 @@ definition irq_opt_relation :: "irq option \<Rightarrow> machine_word \<Rightarr
          Some irq \<Rightarrow> cirq = ucast irq \<and> cirq \<noteq> irqInvalid \<and> irq \<le> Kernel_Config.maxIRQ
        | None \<Rightarrow> cirq = irqInvalid"
 
+lemma irq_opt_relation_Some_ucast:
+  "\<lbrakk> x && mask LENGTH(irq_len) = x;
+     ucast x \<le> (Kernel_Config.maxIRQ :: irq) \<or> x \<le> (Kernel_Config.maxIRQ :: machine_word) \<rbrakk>
+    \<Longrightarrow> irq_opt_relation (Some (ucast x)) (ucast (ucast x::irq))"
+  unfolding irq_opt_relation_def
+  apply (simp add: and_mask_eq_iff_le_mask Kernel_C_maxIRQ)
+  apply (rule conjI, solves \<open>clarsimp simp: irqInvalid_def mask_def unat_arith_simps unat_ucast\<close>)
+  apply (erule disjE, simp)
+  apply (simp add: irq_machine_le_maxIRQ_irq)
+  done
+
+lemma irq_opt_relation_Some_ucast_left:
+  "\<lbrakk> x && mask LENGTH(irq_len) = x;
+     ucast x \<le> (Kernel_Config.maxIRQ :: irq) \<or> x \<le> (Kernel_Config.maxIRQ :: machine_word) \<rbrakk>
+    \<Longrightarrow> irq_opt_relation (Some (ucast x)) x"
+  apply (rule_tac P="irq_opt_relation (Some (ucast x))" in subst[rotated])
+  apply (rule irq_opt_relation_Some_ucast[rotated]; simp)
+  apply word_eqI_solve
+  done
+
 lemma finaliseCap_True_cases_ccorres:
   "\<And>final. isEndpointCap cap \<or> isNotificationCap cap
              \<or> isReplyCap cap \<or> isDomainCap cap \<or> cap = NullCap \<Longrightarrow>
@@ -1728,7 +1748,7 @@ lemma cteDeleteOne_ccorres:
 
 lemma getIRQSlot_ccorres_stuff:
   "\<lbrakk> (s, s') \<in> rf_sr \<rbrakk> \<Longrightarrow>
-   CTypesDefs.ptr_add intStateIRQNode_Ptr (uint (irq :: 10 word))
+   CTypesDefs.ptr_add intStateIRQNode_Ptr (uint (irq ::irq))
      = Ptr (irq_node' s + 2 ^ cte_level_bits * ucast irq)"
   apply (clarsimp simp add: rf_sr_def cstate_relation_def Let_def
                             cinterrupt_relation_def)
@@ -1768,9 +1788,10 @@ lemma deletingIRQHandler_ccorres:
                         ghost_assertion_data_set_def)
   apply (simp add: cap_tag_defs)
   apply (clarsimp simp: cte_wp_at_ctes_of Collect_const_mem
-                        irq_opt_relation_def Kernel_C.maxIRQ_def)
+                        irq_opt_relation_def)
   apply (drule word_le_nat_alt[THEN iffD1])
-  apply (clarsimp simp: uint_0_iff unat_gt_0 uint_up_ucast is_up)
+  apply unat_arith (* only word type bounds should be left *)
+  apply simp
   done
 
 lemma Zombie_new_spec:
@@ -2849,7 +2870,7 @@ lemma finaliseCap_ccorres:
    apply (rule ccorres_if_lhs)
     apply (simp add: Collect_False Collect_True Let_def
                 del: Collect_const)
-    apply (rule_tac P="(capIRQ cap) \<le>  ARM_HYP.maxIRQ" in ccorres_gen_asm)
+    apply (rule_tac P="capIRQ cap \<le> Kernel_Config.maxIRQ" in ccorres_gen_asm)
     apply (rule ccorres_rhs_assoc)+
     apply csymbr
     apply csymbr
@@ -2909,25 +2930,20 @@ lemma finaliseCap_ccorres:
     apply clarsimp
     apply (frule cap_get_tag_to_H, erule(1) cap_get_tag_isCap [THEN iffD2])
     apply (frule(1) ccap_relation_IRQHandler_mask)
-    apply (clarsimp simp: isCap_simps irqInvalid_def
-                          valid_cap'_def ARM_HYP.maxIRQ_def
-                          Kernel_C.maxIRQ_def)
-    apply (rule irq_opt_relation_Some_ucast_left, simp)
-    apply (clarsimp simp: isCap_simps irqInvalid_def
-                          valid_cap'_def ARM_HYP.maxIRQ_def
-                          Kernel_C.maxIRQ_def)
+    apply (clarsimp simp: isCap_simps valid_cap'_def Kernel_C_maxIRQ)
+    apply (rule irq_opt_relation_Some_ucast_left, simp add: irq_len_val)
+    apply (clarsimp simp: isCap_simps valid_cap'_def)
    apply fastforce
   apply clarsimp
   apply (frule cap_get_tag_to_H, erule(1) cap_get_tag_isCap [THEN iffD2])
   apply (frule(1) ccap_relation_IRQHandler_mask)
-  apply (clarsimp simp add:mask_eq_ucast_eq)
+  apply (clarsimp simp add:mask_eq_ucast_eq irq_len_val)
   done
 
 lemma checkIRQ_ret_good:
-  "\<lbrace>\<lambda>s. (irq \<le> scast Kernel_C.maxIRQ \<longrightarrow> P s) \<and> Q s\<rbrace> checkIRQ irq \<lbrace>\<lambda>rv. P\<rbrace>, \<lbrace>\<lambda>rv. Q\<rbrace>"
-  apply (clarsimp simp: checkIRQ_def rangeCheck_def maxIRQ_def minIRQ_def)
-  apply (rule hoare_pre,wp)
-  by (clarsimp simp: Kernel_C.maxIRQ_def split: if_split)
+  "\<lbrace>\<lambda>s. (irq \<le> Kernel_Config.maxIRQ \<longrightarrow> P s) \<and> Q s\<rbrace> checkIRQ irq \<lbrace>\<lambda>rv. P\<rbrace>, \<lbrace>\<lambda>rv. Q\<rbrace>"
+  apply (wpsimp simp: checkIRQ_def rangeCheck_def minIRQ_def)
+  by (clarsimp split: if_split)
 
 lemma Arch_checkIRQ_ccorres:
   "ccorres (syscall_error_rel \<currency> (\<lambda>r r'. irq \<le> scast Kernel_C.maxIRQ))
@@ -2937,18 +2953,19 @@ lemma Arch_checkIRQ_ccorres:
   apply (cinit lift: irq_w___unsigned_long_' )
    apply (simp add: rangeCheck_def unlessE_def ARM_HYP.minIRQ_def checkIRQ_def
                     ucast_nat_def word_le_nat_alt[symmetric]
-                    linorder_not_le[symmetric] maxIRQ_def
+                    linorder_not_le[symmetric] Kernel_C_maxIRQ
                     length_ineq_not_Nil hd_conv_nth cast_simps
                del: Collect_const cong: call_ignore_cong)
    apply (rule ccorres_Cond_rhs_Seq)
     apply (rule ccorres_from_vcg_split_throws[where P=\<top> and P'=UNIV])
      apply vcg
     apply (rule conseqPre, vcg)
-    apply (clarsimp simp: throwError_def return_def Kernel_C.maxIRQ_def
+    apply (clarsimp simp: throwError_def return_def Kernel_C_maxIRQ
                           exception_defs syscall_error_rel_def
                           syscall_error_to_H_cases)
-   apply (clarsimp simp: Kernel_C.maxIRQ_def)
-   apply (rule ccorres_return_CE, simp+)
+   apply clarsimp
+   apply (rule ccorres_return_CE; simp)
+  apply (simp add: Kernel_C_maxIRQ)
   done
 
 end
